Finish proof of one reduction step

ironfleet/src/Dafny/Distributed/Concur/Reduction.i.dfy
@@ -85,58 +85,6 @@ module ReductionModule
         }
     }
 
-/*
-    lemma lemma_PerformOneReductionSwap(
-        trace:Trace,
-        db:seq<DistributedSystemState>,
-        first_entry_pos:int
-        ) returns (
-        trace':Trace,
-        db':seq<DistributedSystemState>
-        )
-        requires IsValidDistributedSystemTraceAndBehavior(trace, db);
-        requires 0 <= first_entry_pos < |trace| - 1;
-        requires GetEntryActor(trace[first_entry_pos]) != GetEntryActor(trace[first_entry_pos+1]);
-        requires EntryIsRightMover(trace[first_entry_pos]) || EntryIsLeftMover(trace[first_entry_pos+1]);
-        ensures  IsValidDistributedSystemTraceAndBehavior(trace', db');
-        ensures  forall sb' :: DistributedSystemBehaviorRefinesSpecBehavior(db', sb') && SpecBehaviorStuttersForMoversInTrace(trace', sb')
-                     ==> exists sb :: DistributedSystemBehaviorRefinesSpecBehavior(db, sb) && SpecBehaviorStuttersForMoversInTrace(trace, sb);
-    {
-        var entry1 := trace[first_entry_pos];
-        var entry2 := trace[first_entry_pos+1];
-        var ds1 := db[first_entry_pos];
-        var ds2 := db[first_entry_pos+1];
-        var ds3 := db[first_entry_pos+2];
-
-        trace' := trace[first_entry_pos := entry2][first_entry_pos + 1 := entry1];
-        var ds2' := lemma_MoverCommutativityForEntries(entry1, entry2, ds1, ds2, ds3);
-        db' := db[first_entry_pos + 1 := ds2'];
-
-        forall sb' | DistributedSystemBehaviorRefinesSpecBehavior(db', sb') && SpecBehaviorStuttersForMoversInTrace(trace', sb')
-            ensures exists sb :: DistributedSystemBehaviorRefinesSpecBehavior(db, sb) && SpecBehaviorStuttersForMoversInTrace(trace, sb);
-        {
-            var sb:seq<SpecState>;
-            if EntryIsRightMover(entry1)
-            {
-                assert sb'[first_entry_pos+1] == sb'[first_entry_pos+2];
-                sb := sb'[first_entry_pos + 1 := sb'[first_entry_pos]];
-                assert SpecBehaviorStuttersForMoversInTrace(trace, sb);
-                lemma_RightMoverForwardPreservation(entry1, ds1, ds2, sb[first_entry_pos]);
-                assert DistributedSystemBehaviorRefinesSpecBehavior(db, sb);
-            }
-            else
-            {
-                assert EntryIsLeftMover(entry2);
-                assert sb'[first_entry_pos] == sb'[first_entry_pos+1];
-                sb := sb'[first_entry_pos + 1 := sb'[first_entry_pos+2]];
-                assert SpecBehaviorStuttersForMoversInTrace(trace, sb);
-                lemma_LeftMoverBackwardPreservation(entry2, ds2, ds3, sb[first_entry_pos+1]);
-                assert DistributedSystemBehaviorRefinesSpecBehavior(db, sb);
-            }
-            assert DistributedSystemBehaviorRefinesSpecBehavior(db, sb) && SpecBehaviorStuttersForMoversInTrace(trace, sb);
-        }
-    }
-*/
 
     lemma lemma_PerformMoveRight(
         trace:Trace,
@@ -212,6 +160,105 @@ module ReductionModule
         }
     }
 
+    function RepeatSpecState(s:SpecState, n:int) : seq<SpecState>
+        requires n >= 0;
+        ensures  var r := RepeatSpecState(s, n); |r| == n && forall i :: 0 <= i < n ==> r[i] == s;
+    {
+        if n == 0 then [] else [s] + RepeatSpecState(s, n-1)
+    }
+
+    lemma lemma_AddStuttersForReductionStepHelper1(
+        trace:Trace,
+        db:seq<DistributedSystemState>,
+        begin_entry_pos:int,
+        end_entry_pos:int,
+        pivot:int,
+        trace':Trace,
+        db':seq<DistributedSystemState>,
+        sb':seq<SpecState>,
+        sb:seq<SpecState>,
+        i:int
+        )
+        requires IsValidDistributedSystemTraceAndBehavior(trace, db);
+        requires 0 <= begin_entry_pos < end_entry_pos < |trace|;
+        requires trace[begin_entry_pos].EntryBeginGroup?;
+        requires trace[end_entry_pos].EntryEndGroup?;
+        requires EntriesCompatibleWithReductionUsingPivot(trace[begin_entry_pos+1 .. end_entry_pos], pivot);
+        requires IsValidDistributedSystemTraceAndBehavior(trace', db');
+        requires DistributedSystemBehaviorRefinesSpecBehavior(db', sb');
+        requires trace' == trace[..begin_entry_pos] + [trace[end_entry_pos].reduced_entry] + trace[end_entry_pos+1 ..];
+        requires db' == db[..begin_entry_pos+1] + db[end_entry_pos+1 ..];
+        requires sb ==   sb'[..begin_entry_pos]
+                       + RepeatSpecState(sb'[begin_entry_pos], pivot + 1)
+                       + RepeatSpecState(sb'[begin_entry_pos+1], end_entry_pos - begin_entry_pos - pivot + 1)
+                       + sb'[begin_entry_pos+2..];
+        requires 0 <= i <= begin_entry_pos + pivot;
+
+        ensures  SpecCorrespondence(db[i], sb[i]);
+    {
+        if i <= begin_entry_pos {
+            return;
+        }
+
+        assert i > 0;
+        var ss := sb'[begin_entry_pos];
+
+        lemma_AddStuttersForReductionStepHelper1(trace, db, begin_entry_pos, end_entry_pos, pivot, trace', db', sb', sb, i-1);
+
+        var j := i-1;
+        lemma_RightMoverForwardPreservation(trace[j], db[j], db[j+1], sb[j]);
+        assert sb[i-1] == ss;
+        assert sb[i] == ss;
+    }
+
+    lemma lemma_AddStuttersForReductionStepHelper2(
+        trace:Trace,
+        db:seq<DistributedSystemState>,
+        begin_entry_pos:int,
+        end_entry_pos:int,
+        pivot:int,
+        trace':Trace,
+        db':seq<DistributedSystemState>,
+        sb':seq<SpecState>,
+        sb:seq<SpecState>,
+        i:int
+        )
+        requires IsValidDistributedSystemTraceAndBehavior(trace, db);
+        requires 0 <= begin_entry_pos < end_entry_pos < |trace|;
+        requires trace[begin_entry_pos].EntryBeginGroup?;
+        requires trace[end_entry_pos].EntryEndGroup?;
+        requires EntriesCompatibleWithReductionUsingPivot(trace[begin_entry_pos+1 .. end_entry_pos], pivot);
+        requires IsValidDistributedSystemTraceAndBehavior(trace', db');
+        requires DistributedSystemBehaviorRefinesSpecBehavior(db', sb');
+        requires trace' == trace[..begin_entry_pos] + [trace[end_entry_pos].reduced_entry] + trace[end_entry_pos+1 ..];
+        requires db' == db[..begin_entry_pos+1] + db[end_entry_pos+1 ..];
+        requires sb ==   sb'[..begin_entry_pos]
+                       + RepeatSpecState(sb'[begin_entry_pos], pivot + 1)
+                       + RepeatSpecState(sb'[begin_entry_pos+1], end_entry_pos - begin_entry_pos - pivot + 1)
+                       + sb'[begin_entry_pos+2..];
+        requires begin_entry_pos + pivot < i < |sb|;
+
+        ensures  SpecCorrespondence(db[i], sb[i]);
+        decreases |sb| - i;
+    {
+        if i >= end_entry_pos + 2 {
+            return;
+        }
+        if i == end_entry_pos + 1 {
+            return;
+        }
+
+        assert |db| == |sb|;
+        var ss := sb'[begin_entry_pos];
+        var ss' := sb'[begin_entry_pos+1];
+
+        lemma_AddStuttersForReductionStepHelper2(trace, db, begin_entry_pos, end_entry_pos, pivot, trace', db', sb', sb, i+1);
+
+        lemma_LeftMoverBackwardPreservation(trace[i], db[i], db[i+1], sb[i+1]);
+        assert sb[i] == ss';
+        assert sb[i+1] == ss';
+    }
+
     lemma lemma_AddStuttersForReductionStep(
         trace:Trace,
         db:seq<DistributedSystemState>,
@@ -235,61 +282,52 @@ module ReductionModule
         requires db' == db[..begin_entry_pos+1] + db[end_entry_pos+1 ..];
 
         ensures  DistributedSystemBehaviorRefinesSpecBehavior(db, sb);
-        ensures  forall i :: begin_entry_pos <= i <= end_entry_pos && i != begin_entry_pos + 1 + pivot ==> sb[i] == sb[i+1];
+        ensures  forall i :: begin_entry_pos <= i <= end_entry_pos && i != begin_entry_pos + pivot ==> sb[i] == sb[i+1];
     {
         var entries := trace[begin_entry_pos+1 .. end_entry_pos];
         var ss := sb'[begin_entry_pos];
         var ss' := sb'[begin_entry_pos+1];
 
-        var pivot_pos := begin_entry_pos + 1 + pivot;
-        assert pivot_pos <= end_entry_pos;
+        sb := sb'[..begin_entry_pos] + RepeatSpecState(ss, pivot + 1) + RepeatSpecState(ss', |entries| - pivot + 2) + sb'[begin_entry_pos+2..];
+        assert |sb| == |sb'| + |entries| + 1 == |db|;
 
-        sb := sb'[..begin_entry_pos+1];
-
-        while |sb| <= pivot_pos
-            invariant begin_entry_pos + 1 <= |sb| <= pivot_pos + 1;
-            invariant forall i :: 0 <= i < begin_entry_pos + 1 ==> sb[i] == sb'[i];
-            invariant forall i :: begin_entry_pos + 1 <= i < |sb| ==> sb[i] == ss;
-            invariant last(sb) == ss;
-            invariant forall i :: begin_entry_pos <= i < |sb| - 1 ==> sb[i] == sb[i+1];
-            invariant IsValidSpecBehavior(sb);
+        forall i | begin_entry_pos <= i <= end_entry_pos && i != begin_entry_pos + pivot
+            ensures sb[i] == sb[i+1];
         {
-            sb := sb + [ss];
+            if i < begin_entry_pos + pivot {
+                assert sb[i] == ss;
+                assert sb[i+1] == ss;
+            }
+            else {
+                assert i > begin_entry_pos + pivot;
+                assert sb[i] == ss';
+                assert sb[i+1] == ss';
+            }
         }
 
-        sb := sb + [ss'];
-        assert |sb| == pivot_pos + 2;
-
-        while |sb| < end_entry_pos + 2
-            invariant pivot_pos + 2 <= |sb| <= end_entry_pos + 2;
-            invariant forall i :: 0 <= i < begin_entry_pos + 1 ==> sb[i] == sb'[i];
-            invariant forall i :: begin_entry_pos + 1 <= i <= pivot_pos ==> sb[i] == ss;
-            invariant forall i :: pivot_pos < i < |sb| ==> sb[i] == ss';
-            invariant last(sb) == ss';
-            invariant forall i :: begin_entry_pos <= i < |sb| - 1 && i != begin_entry_pos + 1 + pivot ==> sb[i] == sb[i+1];
-            invariant IsValidSpecBehavior(sb);
+        forall i | 0 <= i < |sb|
+            ensures SpecCorrespondence(db[i], sb[i]);
         {
-            sb := sb + [ss'];
+            if i <= begin_entry_pos + pivot {
+                lemma_AddStuttersForReductionStepHelper1(trace, db, begin_entry_pos, end_entry_pos, pivot, trace', db', sb', sb, i);
+            }
+            else {
+                lemma_AddStuttersForReductionStepHelper2(trace, db, begin_entry_pos, end_entry_pos, pivot, trace', db', sb', sb, i);
+            }
         }
 
-        assert forall i :: begin_entry_pos <= i <= end_entry_pos && i != begin_entry_pos + 1 + pivot ==> sb[i] == sb[i+1];
-
-        ghost var prev_sb := sb;
-        sb := sb + sb'[begin_entry_pos+2..];
         forall i | 0 <= i < |sb| - 1
             ensures SpecNext(sb[i], sb[i+1]) || sb[i] == sb[i+1];
         {
-            if i < |prev_sb| - 1 {
+            if 0 <= i < begin_entry_pos {
             }
-            else if i == |prev_sb| - 1 {
-                assert SpecNext(last(prev_sb), sb'[begin_entry_pos+2]) || last(prev_sb) == sb'[begin_entry_pos+2];
+            else if i < begin_entry_pos + pivot {
+            }
+            else if i < end_entry_pos {
             }
             else {
             }
         }
-
-        assert IsValidSpecBehavior(sb);
-        assume DistributedSystemBehaviorRefinesSpecBehavior(db, sb);
     }
 
     lemma lemma_PerformOneReductionStep(
@@ -315,7 +353,8 @@ module ReductionModule
         requires EntriesReducibleToEntry(trace[begin_entry_pos+1 .. end_entry_pos], trace[end_entry_pos].reduced_entry);
         ensures  IsValidDistributedSystemTraceAndBehavior(trace', db');
         ensures  forall sb' :: DistributedSystemBehaviorRefinesSpecBehavior(db', sb')
-                     ==> exists sb :: DistributedSystemBehaviorRefinesSpecBehavior(db, sb);
+                     ==> exists sb :: DistributedSystemBehaviorRefinesSpecBehavior(db, sb) &&
+                         forall i :: begin_entry_pos <= i <= end_entry_pos && i != begin_entry_pos + pivot ==> sb[i] == sb[i+1];
     {
         var entries := trace[begin_entry_pos+1 .. end_entry_pos];
         var reduced_entry := trace[end_entry_pos].reduced_entry;
@@ -330,11 +369,17 @@ module ReductionModule
         assert db[begin_entry_pos] == db[begin_entry_pos+1];
         assert db[end_entry_pos] == db[end_entry_pos+1];
         assert DistributedSystemNextEntryAction(db'[begin_entry_pos], db'[begin_entry_pos+1], reduced_entry);
+
+        forall i | 0 <= i < |trace'|
+            ensures DistributedSystemNextEntryAction(db'[i], db'[i+1], trace'[i]);
+        {
+        }
+
         assert IsValidDistributedSystemTraceAndBehavior(trace', db');
 
         forall sb' | DistributedSystemBehaviorRefinesSpecBehavior(db', sb')
             ensures exists sb :: DistributedSystemBehaviorRefinesSpecBehavior(db, sb) &&
-                            forall i :: begin_entry_pos <= i <= end_entry_pos && i != begin_entry_pos + 1 + pivot ==> sb[i] == sb[i+1];
+                            forall i :: begin_entry_pos <= i <= end_entry_pos && i != begin_entry_pos + pivot ==> sb[i] == sb[i+1];
         {
             var sb := lemma_AddStuttersForReductionStep(trace, db, begin_entry_pos, end_entry_pos, pivot, trace', db', sb');
         }
